sound

STLCRecord.v
@@ -11,14 +11,19 @@ Inductive Uniq {t : Type} : list t -> Prop :=
 
 Hint Constructors Uniq.
 
+Lemma uniq_app {T} : forall (l1 l2 : list T), Uniq (l1 ++ l2) -> Uniq l1 /\ Uniq l2.
+Proof with auto.
+  induction l1; intros... inversion H; subst. apply IHl1 in H3. inversion H3. split...
+    constructor... intro. contradict H2. apply in_or_app. left...
+Qed.
+
 (* types *)
 Unset Elimination Schemes.
 Inductive type : Type :=
 | TBool : type
 | TNat : type
 | TArrow : type -> type -> type
-| TRecord : forall (li : list id) (lt : list type),
-              Uniq li -> type.
+| TRecord : list id -> list type -> type.
 Set Elimination Schemes.
 (* The issue with induction is that the automatic induction function
  generated does not provide an inductive hypotheses for TRecords.
@@ -27,14 +32,14 @@ Set Elimination Schemes.
 Definition type_rec := 
 fun (P : type -> Prop) (type_rect_tbool : P TBool) (type_rect_tnat : P TNat)
   (type_rect_tarrow : forall t : type, P t -> forall t0 : type, P t0 -> P (TArrow t t0))
-  (type_rect_trecord : forall li lt u, Forall P lt -> P (TRecord li lt u)) =>
+  (type_rect_trecord : forall li lt, Forall P lt -> P (TRecord li lt)) =>
 fix F (t : type) : P t :=
   match t as t0 return (P t0) with
   | TBool => type_rect_tbool
   | TNat => type_rect_tnat
   | TArrow t0 t1 => type_rect_tarrow t0 (F t0) t1 (F t1)
-  | TRecord li lt u =>
-    type_rect_trecord li lt u
+  | TRecord li lt =>
+    type_rect_trecord li lt
                       ((fix forall_rec (lt' : list type)
                           : Forall P lt' :=
                             match lt' with
@@ -59,11 +64,11 @@ Inductive term : Type :=
 | TNum : nat -> term
 | TPlus : term -> term -> term
 | TEqNat : term -> term -> term
-| TLiteral : forall (li : list id) (lv : list term), Uniq li -> term
+| TLiteral : list id -> list term -> term
 | TAccess : term -> id -> term.
 Set Elimination Schemes.
 (* TODO: Fix inductive hypotheses for f8 (TLiteral's induction) *)
-Definition term_rec := fun (P : term -> Prop) (f : forall i : id, P (TVar i))
+Definition term_ind := fun (P : term -> Prop) (f : forall i : id, P (TVar i))
   (f0 : forall t : term, P t -> forall t0 : term, P t0 -> P (TApp t t0))
   (f1 : forall (i : id) (t : type) (t0 : term), P t0 -> P (TLambda i t t0))
   (f2 : P TTrue) (f3 : P TFalse)
@@ -73,7 +78,7 @@ Definition term_rec := fun (P : term -> Prop) (f : forall i : id, P (TVar i))
   (f5 : forall n : nat, P (TNum n))
   (f6 : forall t : term, P t -> forall t0 : term, P t0 -> P (TPlus t t0))
   (f7 : forall t : term, P t -> forall t0 : term, P t0 -> P (TEqNat t t0))
-  (f8 : forall li lv u, Forall P lv -> P (TLiteral li lv u))
+  (f8 : forall li lv, Forall P lv -> P (TLiteral li lv))
   (f9 : forall t : term, P t -> forall i : id, P (TAccess t i)) =>
 fix F (t : term) : P t :=
   match t as t0 return (P t0) with
@@ -86,14 +91,14 @@ fix F (t : term) : P t :=
   | TNum n => f5 n
   | TPlus t0 t1 => f6 t0 (F t0) t1 (F t1)
   | TEqNat t0 t1 => f7 t0 (F t0) t1 (F t1)
-  | TLiteral li lv u => f8 li lv u ((fix forall_rec (lv' : list term)
-                                     : Forall P lv' :=
-                                       match lv' with
-                                         | nil => Forall_nil P
-                                         | v :: rest =>
-                                           Forall_cons v (F v) (forall_rec rest)
-                                       end)
-                                      lv)
+  | TLiteral li lv => f8 li lv ((fix forall_rec (lv' : list term)
+                                 : Forall P lv' :=
+                                   match lv' with
+                                     | nil => Forall_nil P
+                                     | v :: rest =>
+                                       Forall_cons v (F v) (forall_rec rest)
+                                   end)
+                                  lv)
   | TAccess t0 i => f9 t0 (F t0) i
   end.
 
@@ -116,7 +121,7 @@ Inductive value : term -> Prop :=
 | v_true : value TTrue
 | v_false : value TFalse
 | v_nat : forall n, value (TNum n)
-| v_literal : forall li lv u, (Forall value lv) -> value (TLiteral li lv u).
+| v_literal : forall li lv, (Forall value lv) -> value (TLiteral li lv).
 Set Elimination Schemes.
 
 Definition Admitted {T : Type} : T. admit. Qed.
@@ -126,15 +131,15 @@ Definition value_ind := fun (P : term -> Prop)
   (f0 : P TTrue)
   (f1 : P TFalse)
   (f2 : forall n : nat, P (TNum n))
-  (f3 : forall li lv u,
-        Forall P lv -> P (TLiteral li lv u)) =>
+  (f3 : forall li lv,
+        Forall P lv -> P (TLiteral li lv)) =>
   fix F (t : term) (v : value t) {struct v} : P t :=
   match v in (value t0) return (P t0) with
   | v_abs x T t0 => f x T t0
   | v_true => f0
   | v_false => f1
   | v_nat n => f2 n
-  | v_literal li lv u f5 => f3 li lv u ((fix forallrec l (f5 : Forall value l) : Forall P l := 
+  | v_literal li lv f5 => f3 li lv ((fix forallrec l (f5 : Forall value l) : Forall P l := 
      match f5 with
      | Forall_nil => Forall_nil P
      | Forall_cons t ts vt tvs => Forall_cons t (F t vt) (forallrec ts tvs)
@@ -157,7 +162,7 @@ Fixpoint subst (x : id) (s : term) (t : term) : term :=
     | TNum n => TNum n
     | TPlus l r => TPlus (subst x s l) (subst x s r)
     | TEqNat l r => TEqNat (subst x s l) (subst x s r)
-    | TLiteral li lv u => TLiteral li (map (subst x s) lv) u
+    | TLiteral li lv => TLiteral li (map (subst x s) lv)
     | TAccess r i => TAccess (subst x s r) i
   end.
 
@@ -174,8 +179,8 @@ Fixpoint lookup' (i : id) (l : list (id * term)) : option term :=
 Definition lookup i li lv :=
   lookup' i (combine li lv).
 
-Lemma lookup_in : forall i v li lv,
-                    Uniq li -> lookup i li lv = Some v -> In i li.
+Lemma lookup_in_pair : forall i v li lv,
+                    Uniq li -> lookup i li lv = Some v -> In (i,v) (combine li lv).
 Proof with auto.
   intros i v li. generalize dependent i. generalize dependent v.
   induction li; intros; try solve by inversion.
@@ -184,6 +189,12 @@ Proof with auto.
       SCase "i = a". apply beq_id_eq in Heqb. inversion H0. subst...
       SCase "i != a". inversion H; subst. unfold lookup in IHli. right.
         apply (IHli v i lv H4 H0)...
+Qed.
+
+Lemma lookup_in : forall i v li lv,
+                    Uniq li -> lookup i li lv = Some v -> In i li.
+Proof with auto.
+  intros. apply in_combine_l with (l' := lv) (y := v). apply lookup_in_pair...
 Qed.
 
 Lemma in_lookup : forall i v li lv, Uniq li -> In (i,v) (combine li lv) -> lookup i li lv = Some v.
@@ -217,15 +228,16 @@ Inductive step : term -> term -> Prop :=
                           TEqNat (TNum n) (TNum m) ==> TFalse
 | ST_EqNatL : forall l l' r, l ==> l' -> TEqNat l r ==> TEqNat l' r
 | ST_EqNatR : forall l r r', value l -> r ==> r' -> TEqNat l r ==> TEqNat l r'
-| ST_Literal : forall li lv u ri rv i v v' u' u'', value (TLiteral li lv u) ->
+| ST_Literal : forall li lv ri rv i v v', value (TLiteral li lv) ->
+                                               length li = length lv ->
                                                v ==> v' ->
                                                TLiteral (li ++ (i :: ri))
-                                                        (lv ++ (v :: rv)) u' ==>
+                                                        (lv ++ (v :: rv)) ==>
                                                  TLiteral (li ++ (i :: ri))
-                                                          (lv ++ (v' :: rv)) u''
-| ST_Access : forall li lv u i v, value (TLiteral li lv u) ->
+                                                          (lv ++ (v' :: rv))
+| ST_Access : forall li lv i v, value (TLiteral li lv) ->
                                   lookup i li lv = Some v ->
-                                  TAccess (TLiteral li lv u) i ==> v
+                                  TAccess (TLiteral li lv) i ==> v
 | ST_AccessS : forall r r' i, r ==> r' -> TAccess r i ==> TAccess r' i
     where "t1 '==>' t2" := (step t1 t2).
 
@@ -271,15 +283,16 @@ Inductive has_type : context -> term -> type -> Prop :=
 | T_Nat : forall G n, has_type G (TNum n) TNat
 | T_Plus : forall G l r, has_type G l TNat -> has_type G r TNat -> has_type G (TPlus l r) TNat
 | T_EqNat : forall G l r, has_type G l TNat -> has_type G r TNat -> has_type G (TEqNat l r) TBool
-| T_Literal : forall G li lv lt u u',
+| T_Literal : forall G li lv lt,
                 Forall2 (has_type G) lv lt ->
+                Uniq li ->
                 length li = length lv ->
                 length li = length lt ->
-                has_type G (TLiteral li lv u) (TRecord li lt u')
-| T_Access : forall G li lv lt u u' i v T,
-               has_type G (TLiteral li lv u) (TRecord li lt u') ->
+                has_type G (TLiteral li lv) (TRecord li lt)
+| T_Access : forall G li lv lt i v T,
+               has_type G (TLiteral li lv) (TRecord li lt) ->
                In (i,v) (combine li lv) -> In (i,T) (combine li lt) ->
-               has_type G (TAccess (TLiteral li lv u) i) T.
+               has_type G (TAccess (TLiteral li lv) i) T.
 Set Elimination Schemes.
 
 Definition has_type_ind :=
@@ -308,16 +321,20 @@ fun (P : context -> term -> type -> Prop)
         has_type G l TNat ->
         P G l TNat ->
         has_type G r TNat -> P G r TNat -> P G (TEqNat l r) TBool)
-  (f8 : forall (G : context) li (lv : list term) (lt : list type) u u' llv llt,
-          Forall2 (P G) lv lt -> 
-        P G (TLiteral li lv u) (TRecord li lt u'))
+  (f8 : forall (G : context) li (lv : list term) (lt : list type),
+          length li = length lv ->
+          length li = length lt ->
+          Uniq li ->
+          Forall2 (P G) lv lt ->
+          Forall2 (has_type G) lv lt ->
+        P G (TLiteral li lv) (TRecord li lt))
   (f9 : forall (G : context) li (lv : list term)
-          (lt : list type) u u' (i : id) (v : term) 
+          (lt : list type) (i : id) (v : term) 
           (T : type),
-        has_type G (TLiteral li lv u) (TRecord li lt u') ->
-        P G (TLiteral li lv u) (TRecord li lt u') ->
+        has_type G (TLiteral li lv) (TRecord li lt ) ->
+        P G (TLiteral li lv) (TRecord li lt ) ->
         In (i, v) (combine li lv) -> In (i, T) (combine li lt) ->
-        P G (TAccess (TLiteral li lv u) i) T) =>
+        P G (TAccess (TLiteral li lv) i) T) =>
 fix F (c : context) (t : term) (t0 : type) (h : has_type c t t0) {struct h} : P c t t0 :=
   match h in (has_type c0 t1 t2) return (P c0 t1 t2) with
     | T_Var G x T e => f G x T e
@@ -332,8 +349,8 @@ fix F (c : context) (t : term) (t0 : type) (h : has_type c t t0) {struct h} : P 
     | T_Nat G n => f5 G n
     | T_Plus G l r h0 h1 => f6 G l r h0 (F G l TNat h0) h1 (F G r TNat h1)
     | T_EqNat G l r h0 h1 => f7 G l r h0 (F G l TNat h0) h1 (F G r TNat h1)
-    | T_Literal G li lv lt u u' f10 llv llt =>
-      f8 G li lv lt u u' llv llt
+    | T_Literal G li lv lt f10 u llv llt =>
+      f8 G li lv lt llv llt u
          ((fix forallrec term_list type_list
                (f5 : Forall2 (has_type G)
                              term_list type_list) :
@@ -346,9 +363,9 @@ fix F (c : context) (t : term) (t0 : type) (h : has_type c t t0) {struct h} : P 
                  Forall2_cons term type
                               (F G term type ht)
                               (forallrec terms types forall2_rest)
-             end) lv lt f10)
-    | T_Access G li lv lt u u' i v T h0 i0 i1 =>
-      f9 G li lv lt u u' i v T h0 (F G (TLiteral li lv u) (TRecord li lt u') h0) i0 i1
+             end) lv lt f10) f10
+    | T_Access G li lv lt i v T h0 i0 i1 =>
+      f9 G li lv lt i v T h0 (F G (TLiteral li lv) (TRecord li lt) h0) i0 i1
   end.
 
 Tactic Notation "has_type_cases" tactic(first) ident(c) :=
@@ -396,35 +413,34 @@ Proof with eauto.
     exists TFalse...
     inversion H0. exists (TEqNat l x)...
     inversion H. exists (TEqNat x r)...
-  Case "T_Literal".
-    generalize dependent li.
-    induction H; intros; subst...
+  Case "T_Literal". generalize dependent li.
+    induction H2; intros; subst...
     SCase "Inductive".
       destruct H...
       SSCase "value x".
         destruct li; simpl in *; try solve by inversion.
-        inversion u; subst.
-        destruct (IHForall2 li H4)...
+        inversion H3; subst.
+        inversion H0. inversion H1. inversion H4.
+        destruct (IHForall2 H10 li H6 H7 H12)...
         SSSCase "value TLiteral".
           left. (* (TLiteral ((i0, t) :: l)) is a value *)
           apply v_literal; simpl.
           apply Forall_cons...
-          inversion H1...
+          inversion H13...
         SSSCase "exists t' : TLiteral ==> t'".
-          right. inversion H1; subst. inversion H2; subst.
-          exists (TLiteral (i :: li0 ++ i0 :: ri) (x :: lv ++ v' :: rv) u).
+          right. inversion H13; subst. inversion H14; subst.
+          exists (TLiteral (i :: li0 ++ i0 :: ri) (x :: lv ++ v' :: rv)).
           assert (Uniq (i :: li0)).
             SSSSCase "Proof of assertion".
-              constructor... intro. contradict H3. apply in_or_app. left...
-          apply ST_Literal with (li := (i :: li0)) (lv := x :: lv) (u := H5)...
+              destruct (@uniq_app id (i :: li0) (i0 :: ri))...
+          apply ST_Literal with (li := (i :: li0)) (lv := x :: lv)...
             (* first prove that (TLiteral ((i0, t) :: l0)) is a value *)
               apply v_literal. constructor...
-              inversion H7...
+              inversion H15... simpl. rewrite H16...
       SSCase "exists t' : x ==> t'".
         right. inversion H. destruct li; simpl in *; try solve by inversion.
-        exists (TLiteral (i :: li) (x0 :: l) u).
-        apply ST_Literal with (lv := nil) (li := nil) (u' := u) (u'' := u)
-          (v := x) (v' := x0) (u := Uniq_nil)...
+        exists (TLiteral (i :: li) (x0 :: l)).
+        apply ST_Literal with (lv := nil) (li := nil) (v := x) (v' := x0)...
   Case "T_Access".
     destruct IHHt...
     SCase "TLiteral is a value". right. inversion Ht; subst. apply in_lookup in H...
@@ -463,9 +479,9 @@ Inductive appears_free_in : id -> term -> Prop :=
 | AFI_EqNat2 : forall x l r,
                 appears_free_in x r ->
                 appears_free_in x (TEqNat l r)
-| AFI_Record : forall x id t left right,
+| AFI_Record : forall x id t leftI rightI leftT rightT,
                  appears_free_in x t ->
-                 appears_free_in x (TLiteral (left ++ (id, t) :: right))
+                 appears_free_in x (TLiteral (leftI ++ id :: rightI) (leftT ++ t :: rightT))
 | AFI_Access : forall x t id,
                  appears_free_in x t ->
                  appears_free_in x (TAccess t id).
@@ -495,12 +511,13 @@ Proof.
     Case "AFI_Lambda". inversion H1. subst. apply IHappears_free_in in H7.
       apply not_eq_beq_id_false in H. rewrite extend_neq in H7; assumption.
     Case "AFI_Record".
-      admit.
+      inversion H0; subst... apply Forall2_app_inv_l in H3. inversion H3.
+      inversion H1. inversion H2. inversion H7. inversion H9; subst.
+      apply IHappears_free_in with (T := y). assumption.
     Case "AFI_Access".
       inversion H0; subst.
-      apply IHappears_free_in in H3.
-      exact H3.
-Admitted.
+      apply IHappears_free_in in H3. assumption.
+Qed.
 
 Lemma context_invariance : forall gamma gamma' t T,
                              has_type gamma t T ->
@@ -509,13 +526,35 @@ Lemma context_invariance : forall gamma gamma' t T,
 Proof with eauto.
   intros.
   generalize dependent gamma'.
-  has_type_cases (induction H) Case; intros; auto.
+  has_type_cases (induction H) Case; intros; try solve [auto].
   Case "T_Var". apply T_Var. rewrite <- H0...
   Case "T_Lambda". apply T_Lambda. apply IHhas_type. intros x0 Hafi.
     unfold extend. remember (beq_id x x0). destruct b...
   Case "T_App".
     eapply T_App...
-Admitted.
+  Case "T_Literal".
+    eapply T_Literal... generalize dependent li. induction H2; intros...
+    SCase "Inductive". destruct li; try solve by inversion.
+      constructor... apply H. intros. apply H5.
+      apply AFI_Record with (leftI := nil) (leftT := nil)...
+      inversion H3; subst. eapply IHForall2... intros.
+      inversion H4. apply H10. intros. apply H5.
+      inversion H6.
+      apply AFI_Record with (leftI := i :: leftI)
+                              (leftT := x :: leftT)
+                              (rightI := rightI)
+                              (rightT := rightT)...
+  Case "T_Access". eapply T_Access...
+Qed.
+
+Lemma combine_map {A} {B} {C} : forall (f : B -> C) (l1 : list A) (l2 : list B),
+                                  combine l1 (map f l2) = map (fun p =>
+                                                                 (fst p, f (snd p)))
+                                                              (combine l1 l2).
+Proof with auto.
+  intros f l1. induction l1; intros; simpl...
+  Case "Inductive". destruct l2... simpl. rewrite IHl1...
+Qed.
 
 Lemma substitution_preserves_typing : forall gamma x U t t' T,
                                         has_type (extend gamma x U) t T ->
@@ -524,12 +563,12 @@ Lemma substitution_preserves_typing : forall gamma x U t t' T,
 Proof with eauto.
   intros gamma x U t t' T Ht Ht'.
   generalize dependent gamma. generalize dependent T.
-  term_cases (induction t) Case; intros T gamma H; inversion H; subst; simpl...
+  term_cases (induction t) Case; intros T gamma H'; inversion H'; subst; simpl...
   Case "TVar". rename i into y. remember (beq_id x y) as e. destruct e.
-    SCase "x=y". apply beq_id_eq in Heqe. subst. rewrite extend_eq in H2.
-      inversion H2. subst. eapply context_invariance... intros x Hcontra.
-      destruct (free_in_context _ _ T empty Hcontra)... inversion H0.
-    SCase "x<>y". constructor. rewrite extend_neq in H2...
+    SCase "x=y". apply beq_id_eq in Heqe. subst. rewrite extend_eq in H1.
+      inversion H1. subst. eapply context_invariance... intros x Hcontra.
+      destruct (free_in_context _ _ T empty Hcontra)... inversion H.
+    SCase "x<>y". constructor. rewrite extend_neq in H1...
   Case "TLambda". rename i into y. apply T_Lambda.
     remember (beq_id x y) as e. destruct e.
     SCase "x=y". eapply context_invariance... apply beq_id_eq in Heqe. subst.
@@ -539,12 +578,62 @@ Proof with eauto.
       remember (beq_id y z) as e0. destruct e0...
       apply beq_id_eq in Heqe0. subst.
       rewrite <- Heqe...
-  Case "T_Literal".
+  Case "TLiteral". constructor... generalize dependent li. generalize dependent lt.
+    induction H; intros.
+    SCase "base". inversion H2. constructor.
+    SCase "inductive". destruct lt; try solve by inversion. constructor.
+      inversion H2. apply H...
+      inversion H2. destruct li; try solve by inversion. inversion H3.
+      apply IHForall with (li := li)...
+      rewrite map_length...
+  Case "TAccess".
+    eapply T_Access with (v := subst x t' v)... inversion H1. subst.
+    rewrite combine_map. apply in_map_iff. exists (i,v)...
 Qed.
+
+Lemma combine_3 {A B C} : forall (x : A) (y : B) (z : C) xs ys zs,
+                    In (x,y) (combine xs ys) ->
+                    In (x,z) (combine xs zs) ->
+                    Uniq xs ->
+                    In (y,z) (combine ys zs).
+Proof with auto.
+  induction xs.
+  Case "base". simpl in *. intros. inversion H.
+  Case "inductive". intros. destruct ys; try solve by inversion.
+    destruct zs; try solve by inversion. simpl in *.
+    inversion H; inversion H0; try solve by inversion.
+    inversion H2; inversion H3; subst.
+    left...
+    inversion H2; subst. inversion H1. subst.
+    contradict H6. apply (in_combine_l xs zs x z)...
+    inversion H3; subst. inversion H1. subst.
+    contradict H6. apply (in_combine_l xs ys x y)...
+    right. inversion H1. apply IHxs...
+Qed.
+
+Lemma Forall2_combine_in {A B} : forall P (x : A) (y : B) xs ys,
+                                   In (x,y) (combine xs ys) ->
+                                   Forall2 P xs ys ->
+                                   P x y.
+Proof with auto.
+  intros. induction H0; try solve by inversion.
+  Case "Inductive". simpl in H.  inversion H...
+  inversion H2; subst...
+Qed.
+
+Lemma combine_app {A B} : forall l1 l2 l3 l4 (x : A) (y : B),
+                      length l1 = length l2 ->
+                      (combine l1 l2) ++ (@combine A B l3 l4) = combine (l1 ++ l3) (l2 ++ l4).
+Proof with auto.
+  intros. inversion H.
+  generalize dependent l2.
+  induction l1; intros; destruct l2; try solve by inversion...
+  Case "Inductive". simpl. rewrite IHl1...
+Qed.  
 
 Theorem preservation : forall t t' T,
                          has_type empty t T ->
-                         t => t' ->
+                         t ==> t' ->
                          has_type empty t' T.
 Proof with eauto.
   remember empty as gamma.
@@ -559,6 +648,37 @@ Proof with eauto.
     SCase "ST_AppAbs".
       apply substitution_preserves_typing with T11...
       inversion HT1...
+  Case "T_Literal". inversion HE; subst. constructor...
+    SCase "types match up". generalize dependent lt. generalize dependent li0.
+      induction lv0; intros.
+      SSCase "Base". simpl in *.
+        destruct lt; try solve by inversion...
+        constructor...
+        inversion H2. subst. apply H10...
+        inversion H3...
+      SSCase "Inductive". destruct li0; try solve by inversion.
+        destruct lt; try solve by inversion. constructor...
+        inversion H3... inversion H6. inversion H5. eapply IHlv0...
+        inversion H1...
+        inversion H2...
+        inversion H3...
+        rewrite app_length in *. rewrite app_length in * ... 
+  Case "T_Access". inversion HE; subst... inversion HT; subst.
+    SCase "literal is value".
+      apply lookup_in_pair in H6... 
+      apply Forall2_combine_in with (xs := lv) (ys := lt)...
+      apply combine_3 with (xs := li) (x := i)...
+    SCase "literal steps". inversion H4; subst. apply IHHT in H4...
+      inversion H4. subst.
+      remember (beq_id i i0); destruct b...
+      SSCase "i=i0". apply beq_id_eq in Heqb; subst.
+        apply T_Access with (v := v') (lt := lt)...
+        rewrite <- combine_app... apply in_or_app. right. simpl...
+      SSCase "i!=i0". apply T_Access with (v := v) (lt := lt)...
+        rewrite <- combine_app... rewrite <- combine_app in H...
+        apply in_or_app... apply in_app_or in H. inversion H...
+        right. simpl in *. right. inversion H1... inversion H2. subst.
+        rewrite <- beq_id_refl in Heqb. inversion Heqb.
 Qed.
 
 Definition normal_form {X:Type} (R:relation X) (t:X) : Prop :=
@@ -570,7 +690,7 @@ Definition stuck (t : term) : Prop :=
 
 Corollary soundness : forall t t' T,
   has_type empty t T -> 
-  t =>* t' ->
+  t ==>* t' ->
   ~(stuck t').
 Proof with auto.
   intros t t' T Hhas_type Hmulti. unfold stuck.
